Veritas.Verifier.Correctness.fst
@@ -22,7 +22,7 @@ module E = Veritas.EAC
 module V = Veritas.Verifier
 module VT = Veritas.Verifier.Thread
 module VG = Veritas.Verifier.Global
-
+module TL = Veritas.Verifier.TSLog
 
 //Allow the solver to unroll recursive functions at most once (fuel)
 //Allow the solver to invert inductive definitions at most once (ifuel)
@@ -32,7 +32,7 @@ module VG = Veritas.Verifier.Global
  * an indexed version of time sequence where we track the source verifier thread 
  * for every log entry 
  *)
-let time_seq_idx (gl: VG.hash_verifiable_log): its_hash_verifiable_log (S.length gl) =
+let time_seq_idx (gl: VG.hash_verifiable_log): TL.hash_verifiable_log (S.length gl) =
   admit()
   //interleaved_idx_seq gl (time_seq_ctor gl)
 
@@ -41,7 +41,7 @@ let to_state_op_gvlog (gl: g_vlog) =
   map to_state_op_vlog gl
 
 let lemma_time_seq_rw_consistent (#n:pos) 
-  (itsl: its_hash_verifiable_log n{~ (rw_consistent (to_state_op_vlog (project_seq itsl)))})
+  (itsl: TL.hash_verifiable_log n{~ (rw_consistent (to_state_op_vlog (project_seq itsl)))})
   : hash_collision_gen = 
   let tsl = project_seq itsl in  
   let tsle = time_seq_ext itsl in
