Veritas.Verifier.Merkle.fst
@@ -90,11 +90,11 @@ let lemma_proving_ancestor_blum_bit (#p:pos) (itsl: eac_ts_log p) (k:key{k <> Ro
       
 
 let lemma_addm_ancestor_is_proving (#p:pos) (itsl: its_log p {length itsl > 0}):
-  Lemma (requires (TL.is_eac_log (its_prefix itsl (length itsl - 1)) /\
+  Lemma (requires (TL.is_eac_log (prefix itsl (length itsl - 1)) /\
                    AddM? (its_vlog_entry itsl (length itsl - 1))))
         (ensures (Root <> V.key_of (its_vlog_entry itsl (length itsl - 1)) /\        
                   AddM?.k' (its_vlog_entry itsl (length itsl - 1)) = 
-                  proving_ancestor (its_prefix itsl (length itsl - 1))
+                  proving_ancestor (prefix itsl (length itsl - 1))
                                    (V.key_of (its_vlog_entry itsl (length itsl - 1))))) = admit()
 
  let lemma_store_contains_proving_ancestor (#p:pos) (itsl: eac_ts_log p) 
